Add mostly-proven read_range function
This can be used to implement BFILE.shrink more efficiently by only
retrieving the blocks that are being removed instead of those for the
entire file. The proof is complete except for a bit of slogging through
list rewrites that is left as an exercise to the reader.

src/BlockPtr.v
@@ -1006,7 +1006,7 @@ Module BlockPtr (BPtr : BlockPtrSig).
         erewrite listmatch_combine_l_length_r with (a := A) (b := B) (c := C) (prd := P); auto;
         pred_apply' H; cancel)
     | [ H : context [listmatch _ (combine ?A ?B) _] |- context [length ?B] ] =>
-      replace (length B) with (length A) in * by auto
+      replace (length B) with (length A) by auto
 
     | [ H : context [listmatch _ ?A ?b] |- context [length ?b] ] =>
       replace (length b) with (length A) in * by (
@@ -1040,6 +1040,14 @@ Module BlockPtr (BPtr : BlockPtrSig).
         autorewrite with lists in *; try omega; try erewrite snd_pair by eauto
     | [|- context [selN ?l ?n] ] => rewrite listmatch_isolate with (i := n) (a := combine l _);
         autorewrite with lists in *; try rewrite selN_combine; try omega; try erewrite snd_pair by eauto;
+        cbn [fst snd] in *
+    | [H: context [listmatch _ (combine ?l _)] |- context [selN ?l ?n] ] =>
+        rewrite listmatch_isolate with (i := n) (a := combine l _) in H;
+        autorewrite with lists in *; erewrite ?selN_combine in H; try omega; erewrite ?snd_pair by eauto;
+        cbn [fst snd] in *
+    | [H: context [listmatch _ _ ?l] |- context [selN ?l ?n] ] =>
+        rewrite listmatch_isolate with (i := n) (b := l) in H;
+        autorewrite with lists in *; erewrite ?selN_combine in H; try omega; erewrite ?snd_pair by eauto;
         cbn [fst snd] in *
   end.
 
@@ -1283,6 +1291,459 @@ Module BlockPtr (BPtr : BlockPtrSig).
 
   Local Hint Extern 1 ({{_}} Bind (indread _ _ _ _ ) _) => apply indread_ok : prog.
   Opaque indread.
+
+  Definition indread_aligned indlvl lxp (indbns : list waddr) ms :=
+    ForEach bn rest (rev indbns)
+      Hashmap hm
+      Ghost [ F Fm l_part fsl bxp crash m0 sm m ]
+      Loopvar [ ms r ]
+      Invariant
+        LOG.rep lxp F (LOG.ActiveTxn m0 m) ms sm hm *
+        [[ length indbns = length fsl ]] *
+        [[ r = concat (skipn (length rest) l_part) ]] *
+        [[[ m ::: Fm * listmatch (fun x l' => indrep_n_tree indlvl bxp (snd x) # (fst x) l') (combine (rev indbns) (rev fsl)) (rev l_part) ]]]
+      OnCrash crash
+      Begin
+        let^ (ms, blks) <- indread indlvl lxp # bn ms;
+        Ret ^(ms, blks ++ r)
+      Rof ^(ms, nil).
+
+  Hint Rewrite rev_length rev_involutive rev_app_distr : lists.
+
+  Theorem indread_aligned_ok : forall indlvl lxp indbns ms,
+    {< F Fm m0 sm m bxp fsl l_part,
+    PRE:hm
+           LOG.rep lxp F (LOG.ActiveTxn m0 m) ms sm hm *
+           [[[ m ::: (Fm * listmatch (fun x l => indrep_n_tree indlvl bxp (snd x) # (fst x) l) (combine indbns fsl) l_part) ]]] *
+           [[ length fsl = length indbns ]]
+    POST:hm' RET:^(ms, r)
+           LOG.rep lxp F (LOG.ActiveTxn m0 m) ms sm hm' *
+           [[ r = concat l_part ]]
+    CRASH:hm'  LOG.intact lxp F m0 sm hm'
+    >} indread_aligned indlvl lxp indbns ms.
+  Proof.
+    unfold indread_aligned.
+    step.
+    eassign l_part.
+    autorewrite with lists core.
+    rewrite skipn_oob; auto.
+    indrep_n_tree_bound.
+    rewrite <- combine_rev by auto.
+    rewrite listmatch_rev. cancel.
+    assert (length l_part = length fsl) by indrep_n_tree_bound.
+    prestep. norml.
+    denote app as Hr.
+    apply f_equal with (f := @rev _) in Hr.
+    autorewrite with lists in Hr; cbn [rev] in Hr; subst.
+    autorewrite with lists in *.
+    cbn [length] in *.
+    denote listmatch as Hl.
+    erewrite list_isolate with (l := fsl) (d := emp) in Hl, H by eauto.
+    erewrite list_isolate with (l := l_part) (d := nil) in Hl, H by (substl (length l_part); eauto).
+    autorewrite with lists in Hl, H.
+    cbn [rev app] in Hl, H.
+    repeat rewrite app_assoc_reverse in Hl, H.
+    rewrite combine_app in Hl, H.
+    cbn [app combine] in Hl, H.
+    rewrite listmatch_app_rev, listmatch_cons in Hl.
+    cancel.
+    step.
+    indrep_n_tree_bound.
+    autorewrite with lists core.
+    rewrite skipn_app_r_ge by indrep_n_tree_bound.
+    erewrite skipn_selN_skipn by indrep_n_tree_bound.
+    cbn.
+    autorewrite with core lists.
+    rewrite min_l by omega.
+    autorewrite with core.
+    rewrite firstn_rev by auto.
+    autorewrite with lists core.
+    replace (length l_part - length prefix) with (S (length lst')) by omega.
+    auto.
+    rewrite <- listmatch_app, listmatch_cons.
+    cancel.
+    cancel.
+    auto using LOG.active_intact.
+    left.
+    autorewrite with core lists.
+    rewrite Min.min_assoc, Nat.min_id.
+    congruence.
+    indrep_n_tree_bound.
+    indrep_n_tree_bound.
+    step.
+    eauto using LOG.intact_hashmap_subset.
+  Unshelve.
+    all: constructor.
+  Qed.
+
+  Local Hint Extern 1 ({{_}} Bind (indread_aligned _ _ _ _ ) _) => apply indread_aligned_ok : prog.
+
+  Fixpoint indread_to_aligned indlvl lxp ir start ms :=
+    let N := (NIndirect ^ S indlvl) in
+    If (addr_eq_dec ir 0) {
+      Ret ^(ms, repeat $0 (N - start))
+    } else {
+      let^ (ms, indbns) <- IndRec.read lxp ir 1 ms;
+      match indlvl with
+      | 0 =>
+        Ret ^(ms, skipn start indbns)
+      | S indlvl' =>
+        let N := (NIndirect ^ S indlvl') in
+        let^ (ms, r) <- indread_aligned indlvl' lxp (skipn (S (start / N)) indbns) ms;
+        let ir' := selN indbns (start / N) $0 in
+        let^ (ms, r') <- indread_to_aligned indlvl' lxp # ir' (start mod N) ms;
+        Ret ^(ms, r' ++ r)
+      end
+    }.
+
+  Theorem indread_to_aligned_ok : forall indlvl lxp ir start ms,
+    let N := NIndirect ^ S indlvl in
+    {< F Fm IFs m0 sm m bxp l,
+    PRE:hm
+           LOG.rep lxp F (LOG.ActiveTxn m0 m) ms sm hm *
+           [[[ m ::: Fm * indrep_n_tree indlvl bxp IFs ir l ]]] *
+           [[ start < length l ]]
+    POST:hm' RET:^(ms, r)
+           LOG.rep lxp F (LOG.ActiveTxn m0 m) ms sm hm' *
+           [[ r = skipn start l ]]
+    CRASH:hm'  LOG.intact lxp F m0 sm hm'
+    >} indread_to_aligned indlvl lxp ir start ms.
+  Proof.
+    induction indlvl; cbn [indread_to_aligned].
+    - hoare.
+      rewrite indrep_n_helper_0 in *; destruct_lifts.
+      autorewrite with core.
+      rewrite skipn_repeat; auto.
+      rewrite indrep_n_helper_valid by auto.
+      cancel.
+      rewrite firstn_oob by indrep_n_tree_bound.
+      auto.
+    - step.
+      step.
+      erewrite indrep_n_tree_repeat_concat with (m := list2nmem m).
+      3: pred_apply; cancel.
+      rewrite skipn_repeat; eauto.
+      indrep_n_tree_bound.
+      step.
+      rewrite indrep_n_helper_valid by auto. cancel.
+      rewrite firstn_oob by indrep_n_tree_bound.
+      step.
+      match goal with |- context [skipn ?k] =>
+        rewrite listmatch_split with (n := S k)
+      end.
+      rewrite skipn_combine by auto.
+      cancel.
+      repeat match goal with |- context [match ?x with _ => _ end] => destruct x end;
+        cbn [length] in *; autorewrite with core; congruence.
+      step.
+      indrep_n_extract. cancel.
+      indrep_n_tree_bound.
+      indrep_n_tree_bound.
+      eapply lt_le_trans; [eapply Nat.mod_upper_bound|]; auto.
+      indrep_n_extract.
+      erewrite indrep_n_length_pimpl in *.
+      destruct_lifts.
+      match goal with H: context [selN] |- _ => rewrite H; omega end.
+      indrep_n_tree_bound.
+      indrep_n_tree_bound.
+      step.
+      erewrite <- skipn_hom_concat by eauto.
+      auto.
+  Unshelve.
+    all: solve [eauto | exact $0].
+  Qed.
+
+  Opaque indread_to_aligned.
+  Local Hint Extern 1 ({{_}} Bind (indread_to_aligned _ _ _ _ _ ) _) => apply indread_to_aligned_ok : prog.
+
+  Fixpoint indread_from_aligned indlvl lxp ir len ms :=
+    let N := (NIndirect ^ S indlvl) in
+    If (addr_eq_dec ir 0) {
+      Ret ^(ms, repeat $0 len)
+    } else {
+      let^ (ms, indbns) <- IndRec.read lxp ir 1 ms;
+      match indlvl with
+      | 0 =>
+        Ret ^(ms, firstn len indbns)
+      | S indlvl' =>
+        let N := (NIndirect ^ S indlvl') in
+        let^ (ms, r) <- indread_aligned indlvl' lxp (firstn (len / N) indbns) ms;
+        If (addr_eq_dec (len mod N) 0) {
+          Ret ^(ms, r)
+        } else {
+          let ir' := selN indbns (len / N) $0 in
+          let^ (ms, r') <- indread_from_aligned indlvl' lxp # ir' (len mod N) ms;
+          Ret ^(ms, r ++ r')
+        }
+      end
+    }.
+
+
+  Theorem indread_from_aligned_ok : forall indlvl lxp ir len ms,
+    let N := NIndirect ^ S indlvl in
+    {< F Fm IFs m0 sm m bxp l,
+    PRE:hm
+           LOG.rep lxp F (LOG.ActiveTxn m0 m) ms sm hm *
+           [[[ m ::: Fm * indrep_n_tree indlvl bxp IFs ir l ]]] *
+           [[ len <= length l ]]
+    POST:hm' RET:^(ms, r)
+           LOG.rep lxp F (LOG.ActiveTxn m0 m) ms sm hm' *
+           [[ r = firstn len l ]]
+    CRASH:hm'  LOG.intact lxp F m0 sm hm'
+    >} indread_from_aligned indlvl lxp ir len ms.
+  Proof.
+    induction indlvl; cbn [indread_from_aligned].
+    + hoare.
+      rewrite indrep_n_helper_0 in *; destruct_lifts.
+      autorewrite with core.
+      rewrite firstn_repeat; auto.
+      rewrite repeat_length in *; omega.
+      rewrite indrep_n_helper_valid by auto.
+      cancel.
+      f_equal.
+      rewrite firstn_oob by indrep_n_tree_bound.
+      auto.
+    + step.
+      step.
+      erewrite indrep_n_tree_repeat_concat with (m := list2nmem m).
+      3: pred_apply; cancel.
+      rewrite firstn_repeat; eauto.
+      indrep_n_tree_bound.
+      indrep_n_tree_bound.
+      step.
+      rewrite indrep_n_helper_valid by auto. cancel.
+      rewrite firstn_oob by indrep_n_tree_bound.
+      step.
+      match goal with |- context [firstn ?k] =>
+        rewrite listmatch_split with (n := k)
+      end.
+      rewrite firstn_combine_comm.
+      cancel.
+      indrep_n_tree_bound.
+      step.
+      step.
+      erewrite <- concat_hom_firstn by eauto.
+      rewrite mul_div by mult_nonzero. auto.
+      denote listmatch as Hl; pose proof Hl.
+      prestep. norml.
+      indrep_n_extract.
+      erewrite indrep_n_length_pimpl in *.
+      destruct_lifts.
+      match goal with H: context [selN] |- _ => rename H into Hr end.
+      cancel; hoare.
+      - rewrite Hr; auto using mod_le_r.
+      - erewrite <- firstn_hom_concat by eauto.
+        auto.
+      - indrep_n_tree_bound.
+        denote le as He.
+        destruct (le_lt_eq_dec _ _ He); subst.
+        indrep_n_tree_bound.
+        rewrite Nat.mod_mul in * by auto.
+        congruence.
+      - indrep_n_tree_bound.
+        denote le as He.
+        destruct (le_lt_eq_dec _ _ He); subst.
+        indrep_n_tree_bound.
+        rewrite Nat.mod_mul in * by auto.
+        congruence.
+  Unshelve.
+    all: solve [eauto | exact $0].
+  Qed.
+
+  Local Hint Extern 1 ({{_}} Bind (indread_from_aligned _ _ _ _ _ ) _) => apply indread_from_aligned_ok : prog.
+
+  Definition indread_multiple_blocks indlvl lxp (indbns : list waddr) start len ms :=
+    let N := NIndirect ^ S indlvl in
+    (* reads up to N blocks if start mod N = 0 *)
+    let^ (ms, rl) <- indread_to_aligned indlvl lxp #(selN indbns (start / N) $0) (start mod N) ms;
+    let start' := start + (N - start mod N) in
+    let len' := len - (N - start mod N) in
+    let^ (ms, rm) <- indread_aligned indlvl lxp (firstn (len' / N) (skipn (start' / N) indbns)) ms;
+    let len'' := len' mod N in
+    let start'' := start' + (len' / N * N) in
+    let^ (ms, rr) <- indread_from_aligned indlvl lxp #(selN indbns (start'' / N) $0) len'' ms;
+    Ret ^(ms, rl ++ (rm ++ rr)).
+
+  Theorem indread_multiple_blocks_ok : forall indlvl lxp indbns start len ms,
+    let N := NIndirect ^ S indlvl in
+    {< F Fm m0 sm m bxp l_part fsl,
+    PRE:hm
+           LOG.rep lxp F (LOG.ActiveTxn m0 m) ms sm hm *
+           [[[ m ::: (Fm * listmatch (fun x l => indrep_n_tree indlvl bxp (snd x) #(fst x) l) (combine indbns fsl) l_part) ]]] *
+           [[ start < length (concat l_part) ]] *
+           [[ (N - start mod N) < len ]] *
+           [[ start + len < length (concat l_part) ]] *
+           [[ length indbns = length fsl ]]
+    POST:hm' RET:^(ms, r)
+           LOG.rep lxp F (LOG.ActiveTxn m0 m) ms sm hm' *
+           [[ r = firstn len (skipn start (concat l_part)) ]]
+    CRASH:hm'  LOG.intact lxp F m0 sm hm'
+    >} indread_multiple_blocks indlvl lxp indbns start len ms.
+  Proof.
+    cbv [indread_multiple_blocks].
+    prestep. norml.
+    denote listmatch as Hl. pose proof Hl.
+    assert (length indbns = length l_part) by indrep_n_tree_bound.
+    cancel.
+    indrep_n_extract. cancel.
+    indrep_n_tree_bound.
+    indrep_n_tree_bound.
+    indrep_n_extract.
+    erewrite indrep_n_length_pimpl in *.
+    destruct_lifts.
+    match goal with H: context [selN] |- _ => rewrite H; auto end.
+    indrep_n_tree_bound.
+    indrep_n_tree_bound.
+    step.
+    match goal with |- context [firstn ?m (skipn ?k _)] =>
+      rewrite listmatch_split with (n := k);
+      rewrite listmatch_split with (n := m) (a := skipn _ _)
+    end.
+    rewrite <- firstn_combine_comm.
+    rewrite <- skipn_combine by eauto.
+    cancel.
+    autorewrite with core. congruence.
+    denote (list2nmem m) as Hm. pose proof Hm.
+    indrep_n_extract.
+    rewrite Nat.div_add in * by auto.
+    hoare.
+    - erewrite indrep_n_length_pimpl in *.
+      destruct_lifts.
+      match goal with H: context [selN] |- _ => rewrite H; auto end.
+    - erewrite <- skipn_selN.
+      rewrite <- firstn_hom_concat by eauto using forall_skipn.
+      erewrite skipn_hom_concat by eauto.
+      indrep_n_extract; [ | solve [indrep_n_tree_bound].. ].
+      erewrite indrep_n_length_pimpl in *; destruct_lifts.
+      rewrite firstn_app.
+      rewrite firstn_oob with (n := len).
+      autorewrite with core.
+      match goal with H: context [selN] |- _ => rewrite H end.
+      f_equal.
+      match goal with |- context [?a mod ?b] => destruct (addr_eq_dec 0 (a mod b));
+        try (substl (a mod b)) end.
+      + cbn [skipn firstn].
+        autorewrite with core.
+        repeat f_equal.
+        match goal with |- context [(?a + ?b) / ?b] =>
+          replace ((a + b) / b) with ((a + 1 * b) / b) by (do 2 f_equal; omega)
+        end.
+        rewrite Nat.div_add, plus_comm; auto.
+      + rewrite <- roundup_eq by auto.
+        unfold roundup.
+        rewrite Nat.div_mul by auto.
+        rewrite divup_eq_div_plus_1 by auto.
+        rewrite plus_comm; auto.
+      + autorewrite with core.
+        match goal with H: context [selN] |- _ => rewrite H end.
+        omega.
+    - apply Nat.div_lt_upper_bound; auto.
+      eapply le_lt_trans.
+      apply plus_le_compat_l, div_mul_le.
+      rewrite plus_assoc_reverse.
+      rewrite le_plus_minus_r by omega.
+      indrep_n_tree_bound.
+    - apply Nat.div_lt_upper_bound; auto.
+      eapply le_lt_trans.
+      apply plus_le_compat_l, div_mul_le.
+      rewrite plus_assoc_reverse.
+      rewrite le_plus_minus_r by omega.
+      indrep_n_tree_bound.
+  Unshelve.
+    all: solve [eauto | apply emp | exact $0].
+  Qed.
+
+  Local Hint Extern 1 ({{_}} Bind (indread_multiple_blocks _ _ _ _ _ _ ) _) => apply indread_multiple_blocks_ok : prog.
+
+  Fixpoint indread_range indlvl lxp (root : addr) start len ms :=
+    let N := NIndirect ^ indlvl in
+    If (addr_eq_dec len 0) {
+      Ret ^(ms, nil)
+    } else {
+      (* not necessary, but it makes the proof much easier *)
+      If (addr_eq_dec (start + len) (NIndirect * N)) {
+        indread_to_aligned indlvl lxp root start ms
+      } else {
+        If (addr_eq_dec root 0) {
+          Ret ^(ms, repeat $0 len)
+        } else {
+          let^ (ms, indbns) <- IndRec.read lxp root 1 ms;
+          match indlvl with
+          | 0 =>
+             Ret ^(ms, firstn len (skipn start indbns))
+          | S indlvl' =>
+            If (le_dec len (N - start mod N)) {
+              indread_range indlvl' lxp #(selN indbns (start / N) $0) (start mod N) len ms
+            } else {
+              indread_multiple_blocks indlvl' lxp indbns start len ms
+            }
+          end
+        }
+      }
+    }.
+
+  Theorem indread_range_ok : forall indlvl lxp ir start len ms,
+  {< F Fm Fs m0 sm m bxp l,
+    PRE:hm
+           LOG.rep lxp F (LOG.ActiveTxn m0 m) ms sm hm *
+           [[[ m ::: Fm * indrep_n_tree indlvl Fs bxp ir l ]]] *
+           [[ start + len <= length l ]]
+    POST:hm' RET:^(ms, r)
+           LOG.rep lxp F (LOG.ActiveTxn m0 m) ms sm hm' *
+           [[ r = firstn len (skipn start l) ]]
+    CRASH:hm'  LOG.intact lxp F m0 sm hm'
+    >} indread_range indlvl lxp ir start len ms.
+  Proof.
+    induction indlvl; cbn [indread_range].
+    + hoare.
+      rewrite firstn_oob; indrep_n_tree_bound.
+      rewrite indrep_n_helper_0 in *.
+      destruct_lifts.
+      rewrite skipn_repeat, firstn_repeat; auto.
+      rewrite repeat_length in *; omega.
+      rewrite indrep_n_helper_valid by auto. cancel.
+      repeat f_equal.
+      apply firstn_oob.
+      indrep_n_tree_bound.
+    + step; step.
+      hoare.
+      rewrite firstn_oob; indrep_n_tree_bound.
+      step.
+      step.
+      erewrite indrep_n_tree_repeat_concat with (m := list2nmem m).
+      3: pred_apply; cancel.
+      rewrite skipn_repeat, firstn_repeat; auto.
+      indrep_n_tree_bound.
+      match goal with H: _ + _ <= length ?l * _ |- _ =>
+        replace (length l) with NIndirect in *; indrep_n_tree_bound
+      end.
+      indrep_n_tree_bound.
+      step.
+      rewrite indrep_n_helper_valid by auto. cancel.
+      rewrite firstn_oob by indrep_n_tree_bound.
+      denote listmatch as Hl. pose proof Hl.
+      step.
+      indrep_n_extract.
+      erewrite indrep_n_length_pimpl in *.
+      destruct_lifts.
+      hoare.
+      erewrite skipn_hom_concat by eauto.
+      rewrite firstn_app_l; auto.
+      match goal with H: context [selN] |- _ => rename H into Hr end.
+      autorewrite with core; rewrite Hr.
+      omega.
+      indrep_n_tree_bound.
+      indrep_n_tree_bound.
+      hoare.
+      indrep_n_tree_bound.
+      match goal with H: _ + _ <= length ?l * _ |- _ =>
+        replace (length l) with NIndirect in *; indrep_n_tree_bound
+      end.
+  Unshelve.
+    apply emp.
+  Qed.
+
+  Local Hint Extern 1 ({{_}} Bind (indread_range _ _ _ _ _ _ ) _) => apply indread_range_ok : prog.
 
   Fixpoint indclear_all indlvl lxp bxp root ms :=
     If (addr_eq_dec root 0) {
@@ -2975,6 +3436,31 @@ Module BlockPtr (BPtr : BlockPtrSig).
       Ret ^(ms, (firstn (IRLen ir) ((IRBlocks ir) ++ indbns ++ dindbns ++ tindbns)))
     }.
 
+  Definition indread_range_helper indlvl lxp bn start len ms :=
+    let localstart := fold_left plus (map (fun i => NIndirect ^ S i) (seq 0 indlvl)) 0 in
+    let maxlen := NIndirect ^ S indlvl in
+    If (lt_dec localstart (start + len)) {
+      If (lt_dec start (localstart + maxlen)) {
+        let start' := start - localstart in
+        let len' := len - (localstart - start) in
+        let len'' := Nat.min len' (maxlen - start') in
+        indread_range indlvl lxp bn start' len'' ms
+      } else {
+        Ret ^(ms, nil)
+      }
+    } else {
+      Ret ^(ms, nil)
+    }.
+
+  Definition read_range lxp ir start len ms :=
+    rdir <- Ret (firstn len (skipn start (IRBlocks ir)));
+    let len := len - (NDirect - start) in
+    let start := start - NDirect in
+    let^ (ms, rind) <- indread_range_helper 0 lxp (IRIndPtr ir) start len ms;
+    let^ (ms, rdind) <- indread_range_helper 1 lxp (IRDindPtr ir) start len ms;
+    let^ (ms, rtind) <- indread_range_helper 2 lxp (IRTindPtr ir) start len ms;
+    Ret ^(ms, rdir ++ rind ++ rdind ++ rtind).
+
   Definition indshrink_helper indlvl lxp bxp bn nl ms :=
     let start := fold_left plus (map (fun i => NIndirect ^ S i) (seq 0 indlvl)) 0 in
     let len := NIndirect ^ S indlvl in
@@ -3094,6 +3580,69 @@ Module BlockPtr (BPtr : BlockPtrSig).
     rewrite <- firstn_sum_split. rewrite firstn_skipn.
     congruence.
   Qed.
+
+  Theorem indread_range_helper_ok : forall lxp bn indlvl start len ms,
+    let localstart := fold_left plus (map (fun i => NIndirect ^ S i) (seq 0 indlvl)) 0 in
+    {< F Fm IFs m0 sm m l bxp,
+    PRE:hm
+           LOG.rep lxp F (LOG.ActiveTxn m0 m) ms sm hm *
+           [[[ m ::: (Fm * indrep_n_tree indlvl bxp IFs bn l) ]]]
+    POST:hm' RET:^(ms, r)
+           LOG.rep lxp F (LOG.ActiveTxn m0 m) ms sm hm' *
+           let len' := (len - (localstart - start)) in
+           [[ r = firstn len' (skipn (start - localstart) l) ]]
+    CRASH:hm'  LOG.intact lxp F m0 sm hm'
+    >} indread_range_helper indlvl lxp bn start len ms.
+  Proof.
+    unfold indread_range_helper.
+    step; indrep_n_tree_extract_lengths; hoare.
+    substl (length l).
+    let H := fresh in
+    edestruct Min.min_spec as [ [? H]|[? H] ]; rewrite H; clear H.
+    omega.
+    omega.
+    let H := fresh in
+    edestruct Min.min_spec as [ [? H]|[? H] ]; rewrite H; clear H.
+    auto.
+    rewrite firstn_oob.
+    rewrite firstn_oob; auto.
+    autorewrite with core.
+    omega.
+    autorewrite with core.
+    omega.
+    rewrite skipn_oob, firstn_nil by omega. auto.
+    rewrite sub_le_eq_0 by omega.
+    auto.
+  Qed.
+
+  Local Hint Extern 1 ({{_}} Bind (indread_range_helper _ _ _ _ _ _ ) _) => apply indread_range_helper_ok : prog.
+
+  Theorem read_range_ok : forall lxp bxp ir start len ms,
+    {< F Fm IFs m0 sm m l,
+    PRE:hm
+           LOG.rep lxp F (LOG.ActiveTxn m0 m) ms sm hm *
+           [[[ m ::: Fm * rep bxp IFs ir l ]]] *
+           [[ start + len <= length l ]]
+    POST:hm' RET:^(ms, r)
+           LOG.rep lxp F (LOG.ActiveTxn m0 m) ms sm hm' *
+           [[ r = firstn len (skipn start l) ]]
+    CRASH:hm' LOG.intact lxp F m0 sm hm'
+    >} read_range lxp ir start len ms.
+  Proof.
+    unfold read_range, rep, indrep.
+    hoare.
+    autorewrite with core.
+    substl l.
+    match goal with H: context [firstn NIndirect ?l] |- _ =>
+      rename l into ind
+    end.
+    rewrite firstn_app.
+    rewrite skipn_app_split.
+    rewrite firstn_app.
+    f_equal.
+    rewrite firstn_double_skipn by omega; auto.
+    (* TODO finish proving this and use read_range to implement BFILE.shrink *)
+  Abort.
 
   Lemma indrec_ptsto_pimpl : forall ibn indrec,
     IndRec.rep ibn indrec =p=> exists v, ibn |-> (v, nil).
